refine: arch-split ADT_H (OTHER ARCHES)
Includes minor updates to rest of Refine.

Signed-off-by: Rafal Kolanski <rafal.kolanski@proofcraft.systems>

proof/refine/ARM_HYP/ArchADT_H.thy
@@ -1,5 +1,6 @@
 (*
  * Copyright 2014, General Dynamics C4 Systems
+ * Copyright 2023, Proofcraft Pty Ltd
  *
  * SPDX-License-Identifier: GPL-2.0-only
  *)
@@ -24,36 +25,42 @@ lemma vm_rights_of_vmrights_map_id[ADT_H_assms, simp]:
   by (auto simp: vm_rights_of_def vmrights_map_def valid_vm_rights_def
                  vm_read_write_def vm_read_only_def vm_kernel_only_def)
 
-(* We expect 'a to be one of {pt_index, vs_index} *)
-definition absPageTable0 ::
-  "(obj_ref \<rightharpoonup> Structures_H.kernel_object) \<Rightarrow> obj_ref \<Rightarrow> 'a::len word \<rightharpoonup> ARM_HYP_A.pte" where
-  "absPageTable0 h a \<equiv> \<lambda>offs.
-   case h (a + (ucast offs << pte_bits)) of
-     Some (KOArch (KOPTE (InvalidPTE))) \<Rightarrow> Some ARM_HYP_A.InvalidPTE
-   | Some (KOArch (KOPTE (PagePTE p small global execNever dev rights))) \<Rightarrow>
-       Some (ARM_HYP_A.PagePTE p small
-                               {x. global \<and> x=Global \<or> \<not>execNever \<and> x = Execute \<or>
-                                   dev \<and> x = Device}
-                               (vm_rights_of rights))
-   | Some (KOArch (KOPTE (PageTablePTE p))) \<Rightarrow>
-       if p \<le> mask ppn_len
-       then Some (ARM_HYP_A.PageTablePTE (ucast p))
-       else None
-   | _ \<Rightarrow> None"
+definition
+  absPageTable :: "(word32 \<rightharpoonup> Structures_H.kernel_object) \<Rightarrow> obj_ref \<Rightarrow>
+                  9 word \<Rightarrow> ARM_HYP_A.pte"
+  where
+  "absPageTable h a \<equiv> %offs.
+   case (h (a + (ucast offs << 3))) of
+     Some (KOArch (KOPTE (ARM_HYP_H.InvalidPTE))) \<Rightarrow> ARM_HYP_A.InvalidPTE
+   | Some (KOArch (KOPTE (ARM_HYP_H.LargePagePTE p c xn rights))) \<Rightarrow>
+       if is_aligned offs 4 then
+         ARM_HYP_A.LargePagePTE p
+           {x. c & x=PageCacheable | xn & x=XNever}
+           (vm_rights_of rights)
+       else ARM_HYP_A.InvalidPTE
+   | Some (KOArch (KOPTE (ARM_HYP_H.SmallPagePTE p c xn rights))) \<Rightarrow>
+       ARM_HYP_A.SmallPagePTE p {x. c & x=PageCacheable |
+                                        xn & x=XNever} (vm_rights_of rights)"
 
-definition absPageTable ::
-  "(obj_ref \<rightharpoonup> Structures_H.kernel_object) \<Rightarrow> pt_type option \<Rightarrow> obj_ref \<rightharpoonup> pt" where
-  "absPageTable h pt_t a \<equiv>
-   case pt_t of
-     Some NormalPT_T \<Rightarrow>
-       if is_aligned a (pt_bits NormalPT_T) \<and> (\<forall>off::pt_index. absPageTable0 h a off \<noteq> None)
-       then Some (NormalPT (\<lambda>off. the (absPageTable0 h a off)))
-       else None
-   | Some VSRootPT_T \<Rightarrow>
-       if is_aligned a (pt_bits VSRootPT_T) \<and> (\<forall>off::vs_index. absPageTable0 h a off \<noteq> None)
-       then Some (VSRootPT (\<lambda>off. the (absPageTable0 h a off)))
-       else None
-   | None \<Rightarrow> None"
+definition
+  absPageDirectory :: "(word32 \<rightharpoonup> Structures_H.kernel_object) \<Rightarrow> obj_ref \<Rightarrow>
+                      11 word \<Rightarrow>  ARM_HYP_A.pde"
+  where
+  "absPageDirectory h a \<equiv> %offs.
+   case (h (a + (ucast offs << 3))) of
+     Some (KOArch (KOPDE (ARM_HYP_H.InvalidPDE))) \<Rightarrow> ARM_HYP_A.InvalidPDE
+   | Some (KOArch (KOPDE (ARM_HYP_H.PageTablePDE p))) \<Rightarrow>
+       ARM_HYP_A.PageTablePDE p
+   | Some (KOArch (KOPDE (ARM_HYP_H.SectionPDE p c xn rights))) \<Rightarrow>
+       ARM_HYP_A.SectionPDE p {x. c & x=PageCacheable |
+                                      xn & x=XNever} (vm_rights_of rights)
+   | Some (KOArch (KOPDE (ARM_HYP_H.SuperSectionPDE p c xn rights))) \<Rightarrow>
+       if is_aligned offs 4 then
+         ARM_HYP_A.SuperSectionPDE p
+           {x. c & x=PageCacheable
+             | xn & x=XNever}
+           (vm_rights_of rights)
+       else ARM_HYP_A.InvalidPDE"
 
 definition absVGIC :: "gicvcpuinterface \<Rightarrow> gic_vcpu_interface" where
   "absVGIC v \<equiv> case v of
@@ -64,48 +71,45 @@ lemma absVGIC_eq[simp]:
   by (simp add: vgic_map_def absVGIC_def gic_vcpu_interface.make_def)
 
 (* Can't pull the whole heap off at once, start with arch specific stuff.*)
-definition absHeapArch ::
-  "(machine_word \<rightharpoonup> kernel_object) \<Rightarrow> (machine_word \<rightharpoonup> pt_type) \<Rightarrow>
-   machine_word \<Rightarrow> arch_kernel_object \<rightharpoonup> arch_kernel_obj" where
-  "absHeapArch h pt_types a \<equiv> \<lambda>ako.
-     case ako of
-       KOASIDPool (ARM_HYP_H.ASIDPool ap) \<Rightarrow>
-         Some (ARM_HYP_A.ASIDPool (\<lambda>w. map_option abs_asid_entry (ap (ucast w))))
-     | KOPTE _ \<Rightarrow>
-         map_option PageTable (absPageTable h (pt_types a) a)
-     | KOVCPU (VCPUObj tcb vgic regs vppimask) \<Rightarrow>
-       Some (VCPU \<lparr> vcpu_vgic   = absVGIC vgic,
+definition
+  absHeapArch :: "(word32 \<rightharpoonup> Structures_H.kernel_object) \<Rightarrow> word32
+                 \<Rightarrow> arch_kernel_object \<rightharpoonup> arch_kernel_obj"
+  where
+  "absHeapArch h a \<equiv> %ako.
+   (case ako of
+     KOASIDPool (ARM_HYP_H.ASIDPool ap) \<Rightarrow>
+       Some (ARM_HYP_A.ASIDPool (\<lambda>w. ap (ucast w)))
+   | KOPTE _ \<Rightarrow>
+       if is_aligned a pt_bits then Some (PageTable (absPageTable h a))
+       else None
+   | KOPDE _ \<Rightarrow>
+       if is_aligned a pd_bits then Some (PageDirectory (absPageDirectory h a))
+       else None
+   | KOVCPU (VCPUObj tcb vgic regs vppimask) \<Rightarrow>
+       Some (VCPU \<lparr> vcpu_tcb    = tcb,
+                    vcpu_vgic   = absVGIC vgic,
                     vcpu_regs   = regs,
-                    vcpu_tcb    = tcb,
-                    vcpu_vppi_masked = vppimask \<rparr>)"
-
-definition mdata_map' ::
-  "(asid \<times> vspace_ref) option \<Rightarrow> (Machine_A.ARM_HYP_A.asid \<times> vspace_ref) option" where
-  "mdata_map' = map_option (\<lambda>(asid, ref). (ucast asid, ref))"
-
-lemma mdata_map'_inv[simp]:
-  "mdata_map' (mdata_map m) = m"
-  by (cases m; simp add: mdata_map_def mdata_map'_def split_def ucast_down_ucast_id is_down)
+                    vcpu_vppi_masked = vppimask \<rparr>))"
 
 fun ArchCapabilityMap :: "arch_capability \<Rightarrow> cap" where
   "ArchCapabilityMap (arch_capability.ASIDPoolCap x y) =
-     cap.ArchObjectCap (arch_cap.ASIDPoolCap x (ucast y))"
+     cap.ArchObjectCap (arch_cap.ASIDPoolCap x y)"
 | "ArchCapabilityMap (arch_capability.ASIDControlCap) =
      cap.ArchObjectCap (arch_cap.ASIDControlCap)"
-| "ArchCapabilityMap (arch_capability.FrameCap word rghts sz d data) =
-     cap.ArchObjectCap (arch_cap.FrameCap word (vm_rights_of rghts) sz d (mdata_map' data))"
-| "ArchCapabilityMap (arch_capability.PageTableCap word pt_t data) =
-     cap.ArchObjectCap (arch_cap.PageTableCap word pt_t (mdata_map' data))"
+| "ArchCapabilityMap (arch_capability.PageCap d word rghts sz data) =
+     cap.ArchObjectCap (arch_cap.PageCap d word (vm_rights_of rghts) sz data)"
+| "ArchCapabilityMap (arch_capability.PageTableCap word data) =
+    cap.ArchObjectCap (arch_cap.PageTableCap word data)"
+| "ArchCapabilityMap (arch_capability.PageDirectoryCap word data) =
+    cap.ArchObjectCap (arch_cap.PageDirectoryCap word data)"
 | "ArchCapabilityMap (arch_capability.VCPUCap v) =
-     cap.ArchObjectCap (arch_cap.VCPUCap v)"
+    cap.ArchObjectCap (arch_cap.VCPUCap v)"
 | "ArchCapabilityMap (arch_capability.SGISignalCap irq target) =
-     cap.ArchObjectCap (arch_cap.SGISignalCap (ucast irq) (ucast target))"
-| "ArchCapabilityMap (arch_capability.SMCCap smc_badge) =
-     cap.ArchObjectCap (arch_cap.SMCCap smc_badge)"
+    cap.ArchObjectCap (arch_cap.SGISignalCap (ucast irq) (ucast target))"
 
 lemma acap_relation_imp_ArchCapabilityMap[ADT_H_assms]:
   "\<lbrakk>wellformed_acap ac; acap_relation ac ac'\<rbrakk> \<Longrightarrow> ArchCapabilityMap ac' = cap.ArchObjectCap ac"
-  by (case_tac ac; simp add: wellformed_cap_simps ucast_down_ucast_id is_down)
+  by (case_tac ac; simp add: wellformed_acap_simps ucast_down_ucast_id is_down)
 
 primrec ArchFaultMap :: "Fault_H.arch_fault \<Rightarrow> ExceptionTypes_A.arch_fault" where
   "ArchFaultMap (ARM_HYP_H.VMFault p m) = ARM_HYP_A.VMFault p m"
@@ -117,50 +121,25 @@ lemma ArchFaultMap_arch_fault_map[ADT_H_assms]:
   "ArchFaultMap (arch_fault_map f) = f"
   by (cases f; simp add: ArchFaultMap_def arch_fault_map_def)
 
+(* no FPU on this architecture *)
 definition ArchTcbMap :: "Structures_H.arch_tcb \<Rightarrow> bool \<Rightarrow> Structures_A.arch_tcb" where
   "ArchTcbMap atcb is_cur_fpu_owner \<equiv>
-    \<lparr> tcb_context = atcbContext atcb, tcb_vcpu = atcbVCPUPtr atcb, tcb_cur_fpu = is_cur_fpu_owner \<rparr>"
+    \<lparr> tcb_context = atcbContext atcb, tcb_vcpu = atcbVCPUPtr atcb \<rparr>"
 
 lemma arch_tcb_relation_imp_ArchTcbMap:
-  "\<lbrakk> arch_tcb_relation atcb atcb'; tcb_cur_fpu atcb = is_cur_fpu_owner\<rbrakk>
+  "\<lbrakk> arch_tcb_relation atcb atcb' \<rbrakk>
    \<Longrightarrow> ArchTcbMap atcb' is_cur_fpu_owner = atcb"
   by (clarsimp simp: arch_tcb_relation_def ArchTcbMap_def)
-
-lemma unaligned_page_offsets_helper:
-  "\<lbrakk>is_aligned y (pageBitsForSize vmpage_size); n\<noteq>0;
-    n < 2 ^ (pageBitsForSize vmpage_size - pageBits)\<rbrakk>
-   \<Longrightarrow> \<not> is_aligned (y + n * 2 ^ pageBits :: machine_word) (pageBitsForSize vmpage_size)"
-  apply (simp (no_asm_simp) add: is_aligned_mask)
-  apply (simp add: mask_add_aligned)
-  apply (cut_tac mask_eq_iff_w2p [of "pageBitsForSize vmpage_size" "n * 2 ^ pageBits"])
-   prefer 2
-   apply (case_tac vmpage_size, simp_all add: word_size bit_simps)
-  apply (cut_tac word_power_nonzero_64[of n pageBits];
-         simp add: word_bits_conv pageBits_def)
-   prefer 2
-   apply (case_tac vmpage_size, simp_all add: bit_simps word_size)
-     apply (frule less_trans[of n _ "0x10000000000000"], simp+)+
-  apply clarsimp
-  apply (case_tac vmpage_size, simp_all add: bit_simps)
-    apply (frule_tac i=n and k="0x1000" in word_mult_less_mono1, simp+)+
-  done
 
 definition absArchState ::
   "Arch.kernel_state \<Rightarrow> (obj_ref \<rightharpoonup> arch_kernel_object) \<Rightarrow> arch_state"
   where
   "absArchState s' aobjs' \<equiv>
-   case s' of
-     ARMKernelState asid_tbl kvspace vmid_tab next_vmid global_us_vspace current_vcpu
-                    num_list_regs gs_pt_types current_fpu_owner \<Rightarrow>
-     \<lparr> arm_asid_table = asid_tbl \<circ> ucast,
-       arm_kernel_vspace = kvspace,
-       arm_asid_map = armKSASIDMap' s' aobjs',
-       arm_vmid_table = map_option ucast \<circ> vmid_tab,
-       arm_next_vmid = next_vmid,
-       arm_us_global_vspace = global_us_vspace,
-       arm_current_vcpu = current_vcpu,
-       arm_gicvcpu_numlistregs = num_list_regs,
-       arm_current_fpu_owner = current_fpu_owner \<rparr>"
+   case s' of ARMKernelState asid_tbl hwat anext am curvcpu vnumlistregs globalpd kvspace \<Rightarrow>
+     \<lparr>arm_asid_table = asid_tbl \<circ> ucast,
+      arm_hwasid_table = hwat, arm_next_asid = anext,
+      arm_asid_map = am, arm_current_vcpu = curvcpu, arm_gicvcpu_numlistregs = vnumlistregs,
+      arm_kernel_vspace = kvspace, arm_us_global_pd = globalpd\<rparr>"
 
 lemma absArchState_correct[ADT_H_assms]:
   "(s,s') \<in> state_relation \<Longrightarrow> absArchState (ksArchState s') (aobjs_of' s') = arch_state s"
@@ -168,8 +147,6 @@ lemma absArchState_correct[ADT_H_assms]:
    apply (simp add: state_relation_def)
   apply (clarsimp simp: arch_state_relation_def absArchState_def
                   split: ARM_HYP_H.kernel_state.splits)
-  apply (simp add: o_assoc flip: map_option_comp2)
-  apply (simp add: o_def ucast_up_ucast_id is_up map_option.identity)
   done
 
 end (* Arch *)
@@ -199,10 +176,29 @@ definition absHeap ::
      | Some KOKernelData \<Rightarrow> undefined \<comment> \<open>forbidden by pspace_relation\<close>
      | Some KOUserData \<Rightarrow> map_option (ArchObj \<circ> DataPage False) (ups x)
      | Some KOUserDataDevice \<Rightarrow> map_option (ArchObj \<circ> DataPage True) (ups x)
-     | Some (KOTCB tcb) \<Rightarrow> Some (TCB (TcbMap tcb (armKSCurFPUOwner aks = Some x)))
+     | Some (KOTCB tcb) \<Rightarrow> Some (TCB (TcbMap tcb False)) \<comment> \<open>no FPU on this arch\<close>
      | Some (KOCTE cte) \<Rightarrow> map_option (\<lambda>sz. absCNode sz h x) (cns x)
-     | Some (KOArch ako) \<Rightarrow> map_option ArchObj (absHeapArch h (gsPTTypes aks) x ako)
+     | Some (KOArch ako) \<Rightarrow> map_option ArchObj (absHeapArch h x ako)
      | None \<Rightarrow> None"
+
+lemma unaligned_page_offsets_helper:
+  "\<lbrakk>is_aligned y (pageBitsForSize vmpage_size); n\<noteq>0;
+    n < 2 ^ (pageBitsForSize vmpage_size - pageBits)\<rbrakk>
+   \<Longrightarrow> \<not> is_aligned (y + n * 2 ^ pageBits :: word32) (pageBitsForSize vmpage_size)"
+  apply (simp (no_asm_simp) add: is_aligned_mask)
+  apply (simp add: mask_add_aligned)
+  apply (cut_tac mask_eq_iff_w2p [of "pageBitsForSize vmpage_size" "n * 2 ^ pageBits"])
+   prefer 2
+   apply (case_tac vmpage_size, simp_all add: pageBits_def word_size)
+  apply (cut_tac word_power_nonzero_32[of n pageBits];
+         simp add: word_bits_conv pageBits_def)
+   prefer 2
+   apply (case_tac vmpage_size, simp_all add: pageBits_def word_size)
+     apply (frule less_trans[of n _ "0x100000"], simp+)+
+  apply clarsimp
+  apply (case_tac vmpage_size, simp_all add: pageBits_def)
+    apply (frule_tac i=n and k="0x1000" in word_mult_less_mono1, simp+)+
+  done
 
 lemma absHeap_correct[ADT_H_2_assms]:
   fixes s' :: kernel_state
@@ -223,69 +219,74 @@ proof -
    and gsCNodes:
     "\<And>a n. (\<exists>cs. kheap s a = Some (CNode n cs) \<and> well_formed_cnode_n n cs) \<longleftrightarrow>
             gsCNodes s' a = Some n"
-   and gsPTs:
-    "\<And>a pt_t. (\<exists>pt. kheap s a = Some (ArchObj (PageTable pt)) \<and> pt_t = pt_type pt) \<longleftrightarrow>
-               gsPTTypes (ksArchState s') a = Some pt_t"
     by (fastforce simp add: ghost_relation_def)+
 
   show "?thesis"
-    supply image_cong_simp [cong del]
+  supply image_cong_simp [cong del]
     apply (rule ext)
     apply (simp add: absHeap_def split: option.splits)
     apply (rule conjI)
     using pspace_relation
-     apply (clarsimp simp: pspace_relation_def pspace_dom_def UNION_eq dom_def Collect_eq)
+     apply (clarsimp simp add: pspace_relation_def pspace_dom_def UNION_eq dom_def Collect_eq)
      apply (erule_tac x=x in allE)
      apply clarsimp
      apply (case_tac "kheap s x", simp)
      apply (erule_tac x=x in allE, clarsimp)
      apply (erule_tac x=x in allE, simp add: Ball_def)
      apply (erule_tac x=x in allE, clarsimp)
-     apply (rename_tac a)
-     apply (case_tac a; simp add: other_obj_relation_def
-                             split: if_split_asm Structures_H.kernel_object.splits)
+
+     apply (case_tac a)
+         apply (simp_all add: other_obj_relation_def
+                       split: if_split_asm Structures_H.kernel_object.splits)
       apply (rename_tac sz cs)
-      apply (clarsimp simp: image_def cte_map_def well_formed_cnode_n_def Collect_eq dom_def)
+      apply (clarsimp simp add: image_def cte_map_def well_formed_cnode_n_def Collect_eq dom_def)
       apply (erule_tac x="replicate sz False" in allE)+
       apply simp
      apply (rename_tac arch_kernel_obj)
-     apply (case_tac arch_kernel_obj; simp add: image_def)
-      apply (erule allE, drule_tac x=0 in bspec, simp, fastforce)
-     apply (erule_tac x=0 in allE, simp add: not_less)
+     apply (case_tac arch_kernel_obj, simp_all add: image_def)
+       apply (erule_tac x=0 in allE, simp)
+      apply (erule_tac x=0 in allE, simp)
+     apply clarsimp
+     apply (erule_tac x=0 in allE, simp add: pageBits_def)
      apply (rename_tac vmpage_size)
-     apply (case_tac vmpage_size; simp add: bit_simps)
+     apply (case_tac vmpage_size, simp_all)
 
-    apply (clarsimp split: kernel_object.splits)
+    apply clarsimp
     apply (intro conjI impI allI)
            apply (erule pspace_dom_relatedE[OF _ pspace_relation])
            apply clarsimp
-           apply (case_tac ko; simp add: tcb_relation_cut_def other_obj_relation_def)
-             apply (clarsimp simp: cte_relation_def split: if_split_asm)
-            apply (clarsimp simp: ep_relation_def EndpointMap_def
-                            split: Structures_A.endpoint.splits)
-           apply (clarsimp simp: EndpointMap_def split: Structures_A.endpoint.splits)
+           apply (case_tac ko, simp_all add: tcb_relation_cut_def other_obj_relation_def)
+             apply (clarsimp simp add: cte_relation_def split: if_split_asm)
+            apply (clarsimp simp add: ep_relation_def EndpointMap_def
+                               split: Structures_A.endpoint.splits)
+           apply (clarsimp simp add: EndpointMap_def
+                              split: Structures_A.endpoint.splits)
            apply (rename_tac arch_kernel_obj)
-           apply (case_tac arch_kernel_obj; simp add: other_obj_relation_def)
-            apply (clarsimp simp add: pte_relation_def)
+           apply (case_tac arch_kernel_obj, simp_all add: other_obj_relation_def)
+             apply (clarsimp simp add: pte_relation_def)
+            apply (clarsimp simp add: pde_relation_def)
            apply (clarsimp split: if_split_asm)+
 
           apply (erule pspace_dom_relatedE[OF _ pspace_relation])
-          apply (case_tac ko; simp add: tcb_relation_cut_def other_obj_relation_def)
-            apply (clarsimp simp: cte_relation_def split: if_split_asm)
-           apply (clarsimp simp: ntfn_relation_def AEndpointMap_def
-                           split: Structures_A.ntfn.splits)
-          apply (clarsimp simp: AEndpointMap_def split: Structures_A.ntfn.splits)
+          apply (case_tac ko, simp_all add: tcb_relation_cut_def other_obj_relation_def)
+            apply (clarsimp simp add: cte_relation_def split: if_split_asm)
+           apply (clarsimp simp add: ntfn_relation_def AEndpointMap_def
+                              split: Structures_A.ntfn.splits)
+          apply (clarsimp simp add: AEndpointMap_def
+                             split: Structures_A.ntfn.splits)
           apply (rename_tac arch_kernel_obj)
-          apply (case_tac arch_kernel_obj; simp add: other_obj_relation_def)
-           apply (clarsimp simp add: pte_relation_def)
+          apply (case_tac arch_kernel_obj, simp_all add: other_obj_relation_def)
+            apply (clarsimp simp add: pte_relation_def)
+           apply (clarsimp simp add: pde_relation_def)
           apply (clarsimp split: if_split_asm)+
 
          apply (erule pspace_dom_relatedE[OF _ pspace_relation])
-         apply (case_tac ko; simp add: tcb_relation_cut_def other_obj_relation_def)
-          apply (clarsimp simp: cte_relation_def split: if_split_asm)
+         apply (case_tac ko, simp_all add: tcb_relation_cut_def other_obj_relation_def)
+          apply (clarsimp simp add: cte_relation_def split: if_split_asm)
          apply (rename_tac arch_kernel_obj)
-         apply (case_tac arch_kernel_obj; simp add: other_obj_relation_def)
-          apply (clarsimp simp add: pte_relation_def)
+         apply (case_tac arch_kernel_obj, simp_all add: other_obj_relation_def)
+           apply (clarsimp simp add: pte_relation_def)
+          apply (clarsimp simp add: pde_relation_def)
          apply (clarsimp split: if_split_asm)+
 
         apply (erule pspace_dom_relatedE[OF _ pspace_relation])
@@ -293,55 +294,61 @@ proof -
          apply (clarsimp simp add: cte_relation_def split: if_split_asm)
         apply (rename_tac arch_kernel_obj)
         apply (case_tac arch_kernel_obj, simp_all add: other_obj_relation_def)
-         apply (clarsimp simp add: pte_relation_def)
+          apply (clarsimp simp add: pte_relation_def)
+         apply (clarsimp simp add: pde_relation_def)
         apply (rename_tac vmpage_size)
         apply (cut_tac a=y and sz=vmpage_size in gsUserPages, clarsimp split: if_split_asm)
         apply (case_tac "n=0", simp)
         apply (case_tac "kheap s (y + n * 2 ^ pageBits)")
          apply (rule ccontr)
-         apply (clarsimp simp: shiftl_t2n mult_ac dest!: gsUserPages[symmetric, THEN iffD1] )
+         apply (clarsimp dest!: gsUserPages[symmetric, THEN iffD1] )
     using pspace_aligned
         apply (simp add: pspace_aligned_def dom_def)
         apply (erule_tac x=y in allE)
         apply (case_tac "n=0",(simp split: if_split_asm)+)
         apply (frule (2) unaligned_page_offsets_helper)
         apply (frule_tac y="n*2^pageBits" in pspace_aligned_distinct_None'
-                                             [OF pspace_aligned pspace_distinct])
+                                                [OF pspace_aligned pspace_distinct])
          apply simp
-         apply (rule conjI, clarsimp simp add: word_gt_0)
-         apply (erule n_less_2p_pageBitsForSize)
-        apply (clarsimp simp: shiftl_t2n mult_ac)
+         apply (rule conjI, clarsimp simp add: Word.word_gt_0)
+         apply (simp add: is_aligned_mask)
+         apply (clarsimp simp add: pageBits_def mask_def)
+         apply (case_tac vmpage_size; simp)
+           apply ((frule_tac i=n and k="0x1000" in word_mult_less_mono1, simp+)+)[4]
        apply (erule pspace_dom_relatedE[OF _ pspace_relation])
        apply (case_tac ko, simp_all add: tcb_relation_cut_def other_obj_relation_def)
         apply (clarsimp simp add: cte_relation_def split: if_split_asm)
        apply (rename_tac arch_kernel_obj)
        apply (case_tac arch_kernel_obj, simp_all add: other_obj_relation_def)
-        apply (clarsimp simp add: pte_relation_def)
+         apply (clarsimp simp add: pte_relation_def)
+        apply (clarsimp simp add: pde_relation_def)
        apply (rename_tac vmpage_size)
        apply (cut_tac a=y and sz=vmpage_size in gsUserPages, clarsimp split: if_split_asm)
        apply (case_tac "n=0", simp)
        apply (case_tac "kheap s (y + n * 2 ^ pageBits)")
         apply (rule ccontr)
-        apply (clarsimp simp: shiftl_t2n mult_ac dest!: gsUserPages[symmetric, THEN iffD1])
-       using pspace_aligned
+        apply (clarsimp dest!: gsUserPages[symmetric, THEN iffD1])
+    using pspace_aligned
        apply (simp add: pspace_aligned_def dom_def)
        apply (erule_tac x=y in allE)
        apply (case_tac "n=0",simp+)
        apply (frule (2) unaligned_page_offsets_helper)
        apply (frule_tac y="n*2^pageBits" in pspace_aligned_distinct_None'
-                                         [OF pspace_aligned pspace_distinct])
+                                               [OF pspace_aligned pspace_distinct])
         apply simp
-        apply (rule conjI, clarsimp simp add: word_gt_0)
-        apply (erule n_less_2p_pageBitsForSize)
-       apply (clarsimp simp: shiftl_t2n mult_ac)
-      (* TCB *)
+        apply (rule conjI, clarsimp simp add: Word.word_gt_0)
+        apply (simp add: is_aligned_mask)
+        apply (clarsimp simp add: pageBits_def mask_def)
+        apply (case_tac vmpage_size; simp)
+          apply ((frule_tac i=n and k="0x1000" in word_mult_less_mono1, simp+)+)[4]
       apply (erule pspace_dom_relatedE[OF _ pspace_relation])
       apply (case_tac ko, simp_all add: tcb_relation_cut_def other_obj_relation_def)
         apply (clarsimp simp add: cte_relation_def split: if_split_asm)
        prefer 2
        apply (rename_tac arch_kernel_obj)
        apply (case_tac arch_kernel_obj, simp_all add: other_obj_relation_def)
-        apply (clarsimp simp add: pte_relation_def)
+         apply (clarsimp simp add: pte_relation_def)
+        apply (clarsimp simp add: pde_relation_def)
        apply (clarsimp split: if_split_asm)
       apply (clarsimp simp add: TcbMap_def tcb_relation_def valid_obj_def)
       apply (rename_tac tcb y tcb')
@@ -351,18 +358,15 @@ proof -
       apply (subgoal_tac "map_option FaultMap (tcbFault tcb) = tcb_fault")
        prefer 2
        apply (simp add: fault_rel_optionation_def)
-       using valid_objs[simplified valid_objs_def dom_def fun_app_def, simplified]
+    using valid_objs[simplified valid_objs_def dom_def fun_app_def,simplified]
        apply (erule_tac x=y in allE)
        apply (clarsimp simp: valid_obj_def valid_tcb_def
-                       split: option.splits)
-      using valid_objs[simplified valid_objs_def Ball_def dom_def fun_app_def]
-      apply (erule_tac x=y in allE)
-      using arch_state_relation valid_cur_fpu[simplified valid_cur_fpu_def]
+        split: option.splits)
+    using valid_objs[simplified valid_objs_def Ball_def dom_def fun_app_def]
       apply (erule_tac x=y in allE)
       apply (clarsimp simp add: cap_relation_imp_CapabilityMap valid_obj_def
                                 valid_tcb_def ran_tcb_cap_cases valid_cap_def2
-                                arch_tcb_relation_imp_ArchTcbMap arch_state_relation_def
-                                is_tcb_cur_fpu_def obj_at_def)
+                                arch_tcb_relation_imp_ArchTcbMap)
      apply (simp add: absCNode_def cte_map_def)
      apply (erule pspace_dom_relatedE[OF _ pspace_relation])
      apply (case_tac ko, simp_all add: tcb_relation_cut_def other_obj_relation_def
@@ -370,51 +374,49 @@ proof -
       prefer 2
       apply (rename_tac arch_kernel_obj)
       apply (case_tac arch_kernel_obj, simp_all add: other_obj_relation_def)
-       apply (clarsimp simp add: pte_relation_def)
+        apply (clarsimp simp add: pte_relation_def)
+       apply (clarsimp simp add: pde_relation_def)
       apply (clarsimp split: if_split_asm)
      apply (simp add: cte_map_def)
      apply (clarsimp simp add: cte_relation_def)
      apply (cut_tac a=y and n=sz in gsCNodes, clarsimp)
     using pspace_aligned[simplified pspace_aligned_def]
      apply (drule_tac x=y in bspec, clarsimp)
-     apply clarsimp
-     apply (case_tac "(of_bl ya::machine_word) << cte_level_bits = 0", simp)
+     apply (clarsimp simp: shiftl_t2n')
+     apply (case_tac "(of_bl ya::word32) * 2^cte_level_bits = 0", simp)
       apply (rule ext)
       apply simp
       apply (rule conjI)
        prefer 2
-    using valid_objs[simplified valid_objs_def Ball_def dom_def
-        fun_app_def]
+    using valid_objs[simplified valid_objs_def Ball_def dom_def fun_app_def]
        apply (erule_tac x=y in allE)
        apply (clarsimp simp add: valid_obj_def valid_cs_def valid_cs_size_def
-                   well_formed_cnode_n_def dom_def Collect_eq)
+                                 well_formed_cnode_n_def dom_def Collect_eq)
        apply (frule_tac x=ya in spec, simp)
        apply (erule_tac x=bl in allE)
        apply clarsimp+
       apply (frule pspace_relation_absD[OF _ pspace_relation])
-      apply (simp add: cte_map_def)
+      apply (simp add: cte_map_def shiftl_t2n')
       apply (drule_tac x="y + of_bl bl * 2^cte_level_bits" in spec)
-      apply (clarsimp simp: shiftl_t2n mult_ac)
+      apply clarsimp
       apply (erule_tac x="cte_relation bl" in allE)
       apply (erule impE)
        apply (fastforce simp add: well_formed_cnode_n_def)
       apply clarsimp
       apply (clarsimp simp add: cte_relation_def)
       apply (rule cap_relation_imp_CapabilityMap)
-    using valid_objs[simplified valid_objs_def Ball_def dom_def
-        fun_app_def]
+    using valid_objs[simplified valid_objs_def Ball_def dom_def fun_app_def]
        apply (erule_tac x=y in allE)
        apply (clarsimp simp: valid_obj_def valid_cs_def valid_cap_def2 ran_def)
-       apply (fastforce simp: cte_level_bits_def objBits_defs)+
+       apply (fastforce simp: cte_level_bits_def cteSizeBits_def)+
      apply (subgoal_tac "kheap s (y + of_bl ya * 2^cte_level_bits) = None")
       prefer 2
     using valid_objs[simplified valid_objs_def Ball_def dom_def fun_app_def]
       apply (erule_tac x=y in allE)
       apply (clarsimp simp add: valid_obj_def valid_cs_def valid_cs_size_def)
-      apply (rule pspace_aligned_distinct_None'[OF
-                  pspace_aligned pspace_distinct], assumption)
+      apply (rule pspace_aligned_distinct_None'[OF pspace_aligned pspace_distinct], assumption)
       apply (clarsimp simp: word_neq_0_conv power_add cte_index_repair)
-      apply (simp add: well_formed_cnode_n_def dom_def Collect_eq shiftl_t2n mult_ac)
+      apply (simp add: well_formed_cnode_n_def dom_def Collect_eq)
       apply (erule_tac x=ya in allE)+
       apply (rule word_mult_less_mono1)
         apply (subgoal_tac "sz = length ya")
@@ -424,7 +426,6 @@ proof -
        apply (simp add: cte_level_bits_def)
       apply (simp add: word_bits_conv cte_level_bits_def)
       apply (drule_tac a="2::nat" in power_strict_increasing, simp+)
-     apply (simp add: shiftl_t2n mult_ac)
      apply (rule ccontr, clarsimp)
      apply (cut_tac a="y + of_bl ya * 2^cte_level_bits" and n=yc in gsCNodes)
      apply clarsimp
@@ -435,176 +436,102 @@ proof -
     apply (case_tac ko, simp_all add: tcb_relation_cut_def other_obj_relation_def)
      apply (clarsimp simp add: cte_relation_def split: if_split_asm)
     apply (rename_tac arch_kernel_object y ko P arch_kernel_obj)
-    apply (case_tac arch_kernel_object, simp_all add: absHeapArch_def
-                                            split: asidpool.splits)
+    apply (case_tac arch_kernel_object, simp_all add: absHeapArch_def split: asidpool.splits)
 
-      apply (in_case "KOASIDPool ?pool")
-      apply clarsimp
+       apply clarsimp
+       apply (case_tac arch_kernel_obj)
+           apply (simp add: other_aobj_relation_def asid_pool_relation_def inv_def o_def)
+          apply (clarsimp simp add:  pte_relation_def)
+         apply (clarsimp simp add:  pde_relation_def)
+        apply (clarsimp split: if_split_asm)+
+       apply (clarsimp simp: other_aobj_relation_def)
       apply (case_tac arch_kernel_obj)
-         apply (simp add: other_aobj_relation_def asid_pool_relation_def
-                          inv_def o_def)
+          apply (simp add: other_aobj_relation_def asid_pool_relation_def inv_def o_def)
+    using pspace_aligned[simplified pspace_aligned_def Ball_def dom_def]
+         apply (erule_tac x=y in allE)
+         apply (clarsimp simp add: pte_relation_def absPageTable_def pt_bits_def pageBits_def)
+         apply (rule conjI)
+          prefer 2
+          apply clarsimp
+          apply (rule sym)
+          apply (rule pspace_aligned_distinct_None' [OF pspace_aligned pspace_distinct],
+                 (simp add: vspace_bits_defs)+)
+          apply (cut_tac x=ya and n="2^12" in
+                      ucast_less_shiftl3_helper[where 'a=32,simplified word_bits_conv], simp+)
+          apply (clarsimp simp add: Word.word_gt_0)
+         apply clarsimp
+         apply (subgoal_tac "ucast ya << 3 = 0")
+          prefer 2
+          apply (rule ccontr)
+          apply (frule_tac x=y in unaligned_helper, assumption)
+           apply (rule ucast_less_shiftl3_helper, simp_all add: vspace_bits_defs)
+         apply (rule ext)
+         apply (frule pspace_relation_absD[OF _ pspace_relation])
+         apply simp
+         apply (erule_tac x=offs in allE)
+         apply (clarsimp simp add: pte_relation_def)
+    using valid_objs[simplified valid_objs_def fun_app_def dom_def, simplified]
+         apply (erule_tac x=y in allE)
+         apply (clarsimp simp add: valid_obj_def wellformed_pte_def)
+         apply (erule_tac x=offs in allE)
+         apply (rename_tac pte')
+         apply (case_tac pte', simp_all add: pte_relation_aligned_def vspace_bits_defs)[1]
+          apply (clarsimp split: ARM_HYP_A.pte.splits)
+          apply (rule set_eqI, clarsimp)
+          apply (case_tac x, simp_all)[1]
+         apply (clarsimp split: ARM_HYP_A.pte.splits)
+         apply (rule set_eqI, clarsimp)
+         apply (case_tac x, simp_all)[1]
+        apply (clarsimp simp add: pde_relation_def)
+       apply (clarsimp split: if_split_asm)+
+      apply (simp add: other_aobj_relation_def inv_def o_def)
+     apply (case_tac arch_kernel_obj)
+         apply (simp add: other_aobj_relation_def asid_pool_relation_def inv_def o_def)
         apply (clarsimp simp add:  pte_relation_def)
-       apply (clarsimp simp: other_aobj_relation_def split: if_split_asm)
-      apply (simp add: other_aobj_relation_def)
-
-     apply (in_case "KOPTE ?pte")
-     apply (case_tac arch_kernel_obj;
-            simp add: other_obj_relation_def other_aobj_relation_def asid_pool_relation_def inv_def o_def)
-      apply clarsimp
-      apply (rename_tac p pte pt idx)
-      apply (frule pspace_alignedD, rule pspace_aligned)
-      apply (clarsimp simp add: pte_relation_def)
-      apply (prop_tac "pt_at (pt_type pt) p s", simp add: obj_at_def)
-      apply (drule page_table_at_cross[OF _ pspace_aligned pspace_distinct pspace_relation])
-      apply (clarsimp simp: page_table_at'_def typ_at'_def ko_wp_at'_def)
-      apply (cut_tac a=p and pt_t="pt_type pt" in gsPTs, clarsimp)
-      apply (case_tac "pt_type pt"; clarsimp)
-       apply (in_case "VSRootPT_T")
-       apply (clarsimp simp: absPageTable_def split del: if_split split: option.splits)
-       apply (rule conjI, clarsimp)
+    using pspace_aligned
+       apply (simp add: pspace_aligned_def dom_def)
+       apply (erule_tac x=y in allE)
+       apply (clarsimp simp add: pde_relation_def absPageDirectory_def vspace_bits_defs)
+       apply (rule conjI)
+        prefer 2
+        apply clarsimp
         apply (rule sym)
-        apply (rule pspace_aligned_distinct_None'[OF pspace_aligned pspace_distinct], assumption)
-        apply simp
-        apply (case_tac "idx << pte_bits = 0", simp)
-        apply (clarsimp simp: word_neq_0_conv)
-        apply (rule shiftl_less_t2n)
-         apply (simp add: table_size_def le_mask_iff_lt_2n[THEN iffD1])
-        apply (simp add: table_size_bounded[unfolded word_bits_def, simplified])
-       apply (clarsimp split del: if_split)
-       apply (prop_tac "idx << pte_bits = 0")
-        apply (rename_tac pt_t')
-        apply (cut_tac a="p + (idx << pte_bits)" and pt_t=pt_t' in gsPTs)
-        apply clarsimp
+        apply (rule pspace_aligned_distinct_None' [OF pspace_aligned pspace_distinct],
+               (simp add: vspace_bits_defs)+)
+        apply (cut_tac x=ya and n="2^14" in
+                  ucast_less_shiftl3_helper[where 'a=32, simplified word_bits_conv], simp+)
+        apply (clarsimp simp add: Word.word_gt_0)
+       apply clarsimp
+       apply (subgoal_tac "ucast ya << 3 = 0")
+        prefer 2
         apply (rule ccontr)
-        apply (drule_tac y="idx << pte_bits" in pspace_aligned_distinct_None'
-                                                [OF pspace_aligned pspace_distinct])
-         apply (clarsimp simp: word_neq_0_conv table_size_def)
-         apply (rule shiftl_less_t2n, simp)
-          apply (erule order_le_less_trans)
-          apply (simp add: mask_def bit_simps)
-         apply (simp add: bit_simps)
-        apply simp
-       apply (thin_tac "pte_relation' pte pte'" for pte pte')
-       apply (clarsimp simp: pt_bits_def)
-       apply (case_tac pt; clarsimp)
-       apply (rename_tac vs)
-       apply (clarsimp simp: absPageTable0_def)
-       apply (rule conjI, clarsimp)
-        apply (rule ext, rename_tac offs)
-        apply (erule_tac x="ucast offs" in allE, erule impE, rule ucast_leq_mask)
-         apply (simp add: bit_simps)
-        apply (clarsimp dest!: koTypeOf_pte simp: objBits_simps)
-        apply (erule_tac x="ucast offs" in allE)
-        apply clarsimp
-        apply (rename_tac pte y)
-        apply (frule pspace_relation_absD, rule pspace_relation)
-        apply clarsimp
-        apply (drule_tac x="ucast offs" in bspec)
-         apply clarsimp
-         apply (rule ucast_leq_mask)
-         apply (clarsimp simp: bit_simps)
-        apply (clarsimp simp: pte_relation_def ucast_ucast_mask ge_mask_eq vs_index_bits_def)
-        apply (erule pspace_valid_objsE, rule valid_objs)
-        apply (clarsimp simp: valid_obj_def)
-        apply (erule_tac x=offs in allE)
-        apply (clarsimp simp: wellformed_pte_def)
-        apply (case_tac "vs offs"; clarsimp split: if_split_asm)
-         apply (rule set_eqI, simp)
-         apply (rename_tac x, case_tac x; simp)
-        apply (simp add: ucast_ucast_mask ge_mask_eq)
-        apply clarsimp
-        apply (erule_tac x="ucast off" in allE)
-        apply (erule impE)
-         apply (rule ucast_leq_mask)
-         apply (clarsimp simp: bit_simps)
-        apply (clarsimp dest!: koTypeOf_pte simp: objBits_simps)
-        apply (frule pspace_relation_absD, rule pspace_relation)
-        apply clarsimp
-        apply (drule_tac x="ucast off" in bspec)
-         apply clarsimp
-         apply (rule ucast_leq_mask)
-         apply (clarsimp simp: bit_simps)
-        apply (clarsimp simp: pte_relation_def ucast_ucast_mask ge_mask_eq vs_index_bits_def)
-        apply (case_tac "vs off"; simp add: ucast_leq_mask ppn_len_val)
-
-      (* NormalPT_T is an exact duplicate of the VSRootPT_T case, but I don't see any good way
-         to factor out the commonality *)
-      apply (in_case "NormalPT_T")
-      apply (clarsimp simp: absPageTable_def split del: if_split split: option.splits)
-      apply (rule conjI, clarsimp)
-       apply (rule sym)
-       apply (rule pspace_aligned_distinct_None'[OF pspace_aligned pspace_distinct], assumption)
+        apply (frule_tac x=y in unaligned_helper, assumption)
+         apply (rule ucast_less_shiftl3_helper, simp_all)
+       apply (rule ext)
+       apply (frule pspace_relation_absD[OF _ pspace_relation])
        apply simp
-       apply (case_tac "idx << pte_bits = 0", simp)
-       apply (clarsimp simp: word_neq_0_conv)
-       apply (rule shiftl_less_t2n)
-        apply (simp add: table_size_def le_mask_iff_lt_2n[THEN iffD1])
-       apply (simp add: table_size_bounded[unfolded word_bits_def, simplified])
-      apply (clarsimp split del: if_split)
-      apply (prop_tac "idx << pte_bits = 0")
-       apply (rename_tac pt_t')
-       apply (cut_tac a="p + (idx << pte_bits)" and pt_t=pt_t' in gsPTs)
-       apply clarsimp
-       apply (rule ccontr)
-       apply (drule_tac y="idx << pte_bits" in pspace_aligned_distinct_None'
-                                               [OF pspace_aligned pspace_distinct])
-        apply (clarsimp simp: word_neq_0_conv table_size_def)
-        apply (rule shiftl_less_t2n, simp)
-         apply (erule order_le_less_trans)
-         apply (simp add: mask_def bit_simps)
-        apply (simp add: bit_simps)
-       apply simp
-      apply (thin_tac "pte_relation' pte pte'" for pte pte')
-      apply (clarsimp simp: pt_bits_def)
-      apply (case_tac pt; clarsimp)
-      apply (rename_tac vs)
-      apply (clarsimp simp: absPageTable0_def)
-      apply (rule conjI, clarsimp)
-       apply (rule ext, rename_tac offs)
-       apply (erule_tac x="ucast offs" in allE, erule impE, rule ucast_leq_mask)
-        apply (simp add: bit_simps)
-       apply (clarsimp dest!: koTypeOf_pte simp: objBits_simps)
-       apply (erule_tac x="ucast offs" in allE)
-       apply clarsimp
-       apply (rename_tac pte y)
-       apply (frule pspace_relation_absD, rule pspace_relation)
-       apply clarsimp
-       apply (drule_tac x="ucast offs" in bspec)
-        apply clarsimp
-        apply (rule ucast_leq_mask)
-        apply (clarsimp simp: bit_simps)
-       apply (clarsimp simp: pte_relation_def ucast_ucast_mask ge_mask_eq vs_index_bits_def)
-       apply (erule pspace_valid_objsE, rule valid_objs)
-       apply (clarsimp simp: valid_obj_def)
        apply (erule_tac x=offs in allE)
-       apply (clarsimp simp: wellformed_pte_def)
-       apply (case_tac "vs offs"; clarsimp split: if_split_asm)
-        apply (rule set_eqI, simp)
-        apply (rename_tac x, case_tac x; simp)
-       apply (simp add: ucast_ucast_mask ge_mask_eq)
-      apply clarsimp
-      apply (erule_tac x="ucast off" in allE)
-      apply (erule impE)
-       apply (rule ucast_leq_mask)
-       apply (clarsimp simp: bit_simps)
-      apply (clarsimp dest!: koTypeOf_pte simp: objBits_simps)
-      apply (frule pspace_relation_absD, rule pspace_relation)
-      apply clarsimp
-      apply (drule_tac x="ucast off" in bspec)
-       apply clarsimp
-       apply (rule ucast_leq_mask)
-       apply (clarsimp simp: bit_simps)
-      apply (clarsimp simp: pte_relation_def ucast_ucast_mask ge_mask_eq vs_index_bits_def)
-      apply (case_tac "vs off"; simp add: ucast_leq_mask ppn_len_val)
+       apply (clarsimp simp add: pde_relation_def)
 
-     apply (in_case "DataPage ?p ?sz")
-     apply (clarsimp split: if_splits)
+    using valid_objs[simplified valid_objs_def fun_app_def dom_def,simplified]
+       apply (erule_tac x=y in allE)
+       apply (clarsimp simp add: valid_obj_def wellformed_pde_def vspace_bits_defs)
+       apply (erule_tac x=offs in allE)
+       apply (rename_tac pde')
+       apply (case_tac pde', simp_all add: pde_relation_aligned_def)[1]
+          apply (clarsimp split: ARM_HYP_A.pde.splits)+
+        apply (rule set_eqI, clarsimp)
+        apply (case_tac x, simp_all)[1]
+       apply (clarsimp split: ARM_HYP_A.pde.splits)
+       apply (rule set_eqI, clarsimp)
+       apply (case_tac x, simp_all)[1]
+      apply (clarsimp simp add: pde_relation_def split: if_split_asm)
+     apply (clarsimp simp add: other_aobj_relation_def)
 
-    apply (in_case "KOVCPU ?vcpu")
     apply clarsimp
     apply (rename_tac arch_kernel_obj vcpu)
     apply (case_tac arch_kernel_obj;
-           clarsimp simp: other_obj_relation_def other_aobj_relation_def pte_relation_def split: if_splits)
+           clarsimp simp: other_aobj_relation_def pte_relation_def pde_relation_def split: if_splits)
     apply (rename_tac vcpu')
     apply (case_tac vcpu')
     apply (clarsimp simp: vcpu_relation_def split: vcpu.splits)
