proof/refine/RISCV64/ArchADT_H.thy
@@ -1,5 +1,6 @@
 (*
  * Copyright 2020, Data61, CSIRO (ABN 41 687 119 230)
+ * Copyright 2023, Proofcraft Pty Ltd
  *
  * SPDX-License-Identifier: GPL-2.0-only
  *)
@@ -24,60 +25,36 @@ lemma vm_rights_of_vmrights_map_id[ADT_H_assms, simp]:
   by (auto simp: vm_rights_of_def vmrights_map_def valid_vm_rights_def
                  vm_read_write_def vm_read_only_def vm_kernel_only_def)
 
-(* We expect 'a to be one of {pt_index, vs_index} *)
 definition absPageTable0 ::
-  "(obj_ref \<rightharpoonup> Structures_H.kernel_object) \<Rightarrow> obj_ref \<Rightarrow> 'a::len word \<rightharpoonup> RISCV64_A.pte" where
+  "(obj_ref \<rightharpoonup> Structures_H.kernel_object) \<Rightarrow> obj_ref \<Rightarrow> pt_index \<rightharpoonup> RISCV64_A.pte" where
   "absPageTable0 h a \<equiv> \<lambda>offs.
-   case h (a + (ucast offs << pte_bits)) of
+   case (h (a + (ucast offs << pte_bits))) of
      Some (KOArch (KOPTE (InvalidPTE))) \<Rightarrow> Some RISCV64_A.InvalidPTE
-   | Some (KOArch (KOPTE (PagePTE p small global execNever dev rights))) \<Rightarrow>
-       Some (RISCV64_A.PagePTE p small
-                               {x. global \<and> x=Global \<or> \<not>execNever \<and> x = Execute \<or>
-                                   dev \<and> x = Device}
-                               (vm_rights_of rights))
-   | Some (KOArch (KOPTE (PageTablePTE p))) \<Rightarrow>
+   | Some (KOArch (KOPTE (PagePTE p g u e rights))) \<Rightarrow>
        if p \<le> mask ppn_len
-       then Some (RISCV64_A.PageTablePTE (ucast p))
+       then Some (RISCV64_A.PagePTE (ucast p) {x. g \<and> x=Global \<or> u \<and> x = User \<or> e \<and> x = Execute}
+                                    (vm_rights_of rights))
+       else None
+   | Some (KOArch (KOPTE (PageTablePTE p g))) \<Rightarrow>
+       if p \<le> mask ppn_len
+       then Some (RISCV64_A.PageTablePTE (ucast p) {x. g \<and> x=Global})
        else None
    | _ \<Rightarrow> None"
 
 definition absPageTable ::
-  "(obj_ref \<rightharpoonup> Structures_H.kernel_object) \<Rightarrow> pt_type option \<Rightarrow> obj_ref \<rightharpoonup> pt" where
-  "absPageTable h pt_t a \<equiv>
-   case pt_t of
-     Some NormalPT_T \<Rightarrow>
-       if is_aligned a (pt_bits NormalPT_T) \<and> (\<forall>off::pt_index. absPageTable0 h a off \<noteq> None)
-       then Some (NormalPT (\<lambda>off. the (absPageTable0 h a off)))
-       else None
-   | Some VSRootPT_T \<Rightarrow>
-       if is_aligned a (pt_bits VSRootPT_T) \<and> (\<forall>off::vs_index. absPageTable0 h a off \<noteq> None)
-       then Some (VSRootPT (\<lambda>off. the (absPageTable0 h a off)))
-       else None
-   | None \<Rightarrow> None"
-
-definition absVGIC :: "gicvcpuinterface \<Rightarrow> gic_vcpu_interface" where
-  "absVGIC v \<equiv> case v of
-    VGICInterface hcr vmcr apr lr \<Rightarrow> gic_vcpu_interface.make hcr vmcr apr lr"
-
-lemma absVGIC_eq[simp]:
-  "absVGIC (vgic_map vgic) = vgic"
-  by (simp add: vgic_map_def absVGIC_def gic_vcpu_interface.make_def)
+  "(obj_ref \<rightharpoonup> Structures_H.kernel_object) \<Rightarrow> obj_ref \<rightharpoonup> (pt_index \<Rightarrow> RISCV64_A.pte)" where
+  "absPageTable h a \<equiv>
+     if is_aligned a pt_bits \<and> (\<forall>off. absPageTable0 h a off \<noteq> None)
+     then Some (\<lambda>off. the (absPageTable0 h a off))
+     else None"
 
 (* Can't pull the whole heap off at once, start with arch specific stuff.*)
 definition absHeapArch ::
-  "(machine_word \<rightharpoonup> kernel_object) \<Rightarrow> (machine_word \<rightharpoonup> pt_type) \<Rightarrow>
-   machine_word \<Rightarrow> arch_kernel_object \<rightharpoonup> arch_kernel_obj" where
-  "absHeapArch h pt_types a \<equiv> \<lambda>ako.
+  "(machine_word \<rightharpoonup> kernel_object) \<Rightarrow> machine_word \<Rightarrow> arch_kernel_object \<rightharpoonup> arch_kernel_obj" where
+  "absHeapArch h a \<equiv> \<lambda>ako.
      case ako of
-       KOASIDPool (RISCV64_H.ASIDPool ap) \<Rightarrow>
-         Some (RISCV64_A.ASIDPool (\<lambda>w. map_option abs_asid_entry (ap (ucast w))))
-     | KOPTE _ \<Rightarrow>
-         map_option PageTable (absPageTable h (pt_types a) a)
-     | KOVCPU (VCPUObj tcb vgic regs vppimask) \<Rightarrow>
-       Some (VCPU \<lparr> vcpu_vgic   = absVGIC vgic,
-                    vcpu_regs   = regs,
-                    vcpu_tcb    = tcb,
-                    vcpu_vppi_masked = vppimask \<rparr>)"
+       KOASIDPool (RISCV64_H.ASIDPool ap) \<Rightarrow> Some (RISCV64_A.ASIDPool (\<lambda>w. ap (ucast w)))
+     | KOPTE _ \<Rightarrow> map_option PageTable (absPageTable h a)"
 
 definition mdata_map' ::
   "(asid \<times> vspace_ref) option \<Rightarrow> (Machine_A.RISCV64_A.asid \<times> vspace_ref) option" where
@@ -94,35 +71,28 @@ fun ArchCapabilityMap :: "arch_capability \<Rightarrow> cap" where
      cap.ArchObjectCap (arch_cap.ASIDControlCap)"
 | "ArchCapabilityMap (arch_capability.FrameCap word rghts sz d data) =
      cap.ArchObjectCap (arch_cap.FrameCap word (vm_rights_of rghts) sz d (mdata_map' data))"
-| "ArchCapabilityMap (arch_capability.PageTableCap word pt_t data) =
-     cap.ArchObjectCap (arch_cap.PageTableCap word pt_t (mdata_map' data))"
-| "ArchCapabilityMap (arch_capability.VCPUCap v) =
-     cap.ArchObjectCap (arch_cap.VCPUCap v)"
-| "ArchCapabilityMap (arch_capability.SGISignalCap irq target) =
-     cap.ArchObjectCap (arch_cap.SGISignalCap (ucast irq) (ucast target))"
-| "ArchCapabilityMap (arch_capability.SMCCap smc_badge) =
-     cap.ArchObjectCap (arch_cap.SMCCap smc_badge)"
+| "ArchCapabilityMap (arch_capability.PageTableCap word data) =
+    cap.ArchObjectCap (arch_cap.PageTableCap word (mdata_map' data))"
 
 lemma acap_relation_imp_ArchCapabilityMap[ADT_H_assms]:
   "\<lbrakk>wellformed_acap ac; acap_relation ac ac'\<rbrakk> \<Longrightarrow> ArchCapabilityMap ac' = cap.ArchObjectCap ac"
   by (case_tac ac; simp add: wellformed_cap_simps ucast_down_ucast_id is_down)
 
 primrec ArchFaultMap :: "Fault_H.arch_fault \<Rightarrow> ExceptionTypes_A.arch_fault" where
-  "ArchFaultMap (RISCV64_H.VMFault p m) = RISCV64_A.VMFault p m"
-| "ArchFaultMap (RISCV64_H.VCPUFault w) = RISCV64_A.VCPUFault w"
-| "ArchFaultMap (RISCV64_H.VGICMaintenance m) = RISCV64_A.VGICMaintenance m"
-| "ArchFaultMap (RISCV64_H.VPPIEvent irq) = RISCV64_A.VPPIEvent irq"
+  "ArchFaultMap (ArchFault_H.RISCV64_H.arch_fault.VMFault p m) =
+     Machine_A.RISCV64_A.arch_fault.VMFault p m"
 
 lemma ArchFaultMap_arch_fault_map[ADT_H_assms]:
   "ArchFaultMap (arch_fault_map f) = f"
   by (cases f; simp add: ArchFaultMap_def arch_fault_map_def)
 
+(* no FPU on this architecture *)
 definition ArchTcbMap :: "Structures_H.arch_tcb \<Rightarrow> bool \<Rightarrow> Structures_A.arch_tcb" where
   "ArchTcbMap atcb is_cur_fpu_owner \<equiv>
-    \<lparr> tcb_context = atcbContext atcb, tcb_vcpu = atcbVCPUPtr atcb, tcb_cur_fpu = is_cur_fpu_owner \<rparr>"
+    \<lparr> tcb_context = atcbContext atcb \<rparr>"
 
 lemma arch_tcb_relation_imp_ArchTcbMap:
-  "\<lbrakk> arch_tcb_relation atcb atcb'; tcb_cur_fpu atcb = is_cur_fpu_owner\<rbrakk>
+  "\<lbrakk> arch_tcb_relation atcb atcb' \<rbrakk>
    \<Longrightarrow> ArchTcbMap atcb' is_cur_fpu_owner = atcb"
   by (clarsimp simp: arch_tcb_relation_def ArchTcbMap_def)
 
@@ -145,22 +115,35 @@ lemma unaligned_page_offsets_helper:
     apply (frule_tac i=n and k="0x1000" in word_mult_less_mono1, simp+)+
   done
 
+lemma pte_offset_in_datapage:
+  "\<lbrakk> n < 2 ^ (pageBitsForSize sz - pageBits); n \<noteq> 0 \<rbrakk> \<Longrightarrow>
+   (n << pageBits) - (ucast off << pte_bits) < 2 ^ pageBitsForSize sz"
+  for n::machine_word and off::pt_index
+  apply (frule n_less_2p_pageBitsForSize)
+  apply (simp only: bit_simps)
+  apply (subst shiftl_t2n)
+  apply (rule order_le_less_trans[rotated], assumption)
+  apply (rule word_le_imp_diff_le)
+   prefer 2
+   apply (simp add: mult_ac)
+  apply (subst shiftl_t2n[symmetric])
+  apply (subst (asm) mult_ac)
+  apply (subst (asm) shiftl_t2n[symmetric])+
+  apply (rule order_trans[where y="mask pageBits"])
+   apply (simp add: le_mask_shiftl_le_mask[where n=9] ucast_leq_mask pageBits_def)
+  apply word_bitwise
+  apply (clarsimp simp: nth_w2p pageBits_def rev_bl_order_simps)
+  apply (cases sz; simp add: pageBits_def ptTranslationBits_def)
+  done
+
 definition absArchState ::
   "Arch.kernel_state \<Rightarrow> (obj_ref \<rightharpoonup> arch_kernel_object) \<Rightarrow> arch_state"
   where
   "absArchState s' aobjs' \<equiv>
-   case s' of
-     ARMKernelState asid_tbl kvspace vmid_tab next_vmid global_us_vspace current_vcpu
-                    num_list_regs gs_pt_types current_fpu_owner \<Rightarrow>
-     \<lparr> arm_asid_table = asid_tbl \<circ> ucast,
-       arm_kernel_vspace = kvspace,
-       arm_asid_map = armKSASIDMap' s' aobjs',
-       arm_vmid_table = map_option ucast \<circ> vmid_tab,
-       arm_next_vmid = next_vmid,
-       arm_us_global_vspace = global_us_vspace,
-       arm_current_vcpu = current_vcpu,
-       arm_gicvcpu_numlistregs = num_list_regs,
-       arm_current_fpu_owner = current_fpu_owner \<rparr>"
+   case s' of RISCVKernelState asid_tbl gpts kvspace \<Rightarrow>
+     \<lparr>riscv_asid_table = asid_tbl \<circ> ucast,
+      riscv_global_pts = \<lambda>l. set (gpts (size l)),
+      riscv_kernel_vspace = kvspace\<rparr>"
 
 lemma absArchState_correct[ADT_H_assms]:
   "(s,s') \<in> state_relation \<Longrightarrow> absArchState (ksArchState s') (aobjs_of' s') = arch_state s"
@@ -168,8 +151,6 @@ lemma absArchState_correct[ADT_H_assms]:
    apply (simp add: state_relation_def)
   apply (clarsimp simp: arch_state_relation_def absArchState_def
                   split: RISCV64_H.kernel_state.splits)
-  apply (simp add: o_assoc flip: map_option_comp2)
-  apply (simp add: o_def ucast_up_ucast_id is_up map_option.identity)
   done
 
 end (* Arch *)
@@ -199,10 +180,16 @@ definition absHeap ::
      | Some KOKernelData \<Rightarrow> undefined \<comment> \<open>forbidden by pspace_relation\<close>
      | Some KOUserData \<Rightarrow> map_option (ArchObj \<circ> DataPage False) (ups x)
      | Some KOUserDataDevice \<Rightarrow> map_option (ArchObj \<circ> DataPage True) (ups x)
-     | Some (KOTCB tcb) \<Rightarrow> Some (TCB (TcbMap tcb (armKSCurFPUOwner aks = Some x)))
+     | Some (KOTCB tcb) \<Rightarrow> Some (TCB (TcbMap tcb False)) \<comment> \<open>no FPU on this arch\<close>
      | Some (KOCTE cte) \<Rightarrow> map_option (\<lambda>sz. absCNode sz h x) (cns x)
-     | Some (KOArch ako) \<Rightarrow> map_option ArchObj (absHeapArch h (gsPTTypes aks) x ako)
+     | Some (KOArch ako) \<Rightarrow> map_option ArchObj (absHeapArch h x ako)
      | None \<Rightarrow> None"
+
+lemma distinct_word_add_inj_ptes:
+  "\<lbrakk> p + (ucast off << pte_bits) = p' + (ucast off' << pte_bits);
+     is_aligned p pt_bits; is_aligned p' pt_bits \<rbrakk>
+   \<Longrightarrow> p' = p \<and> off' = off" for off :: pt_index and p :: machine_word
+  by (erule (2) distinct_word_add_ucast_shift_inj; simp add: bit_simps)
 
 lemma absHeap_correct[ADT_H_2_assms]:
   fixes s' :: kernel_state
@@ -223,9 +210,6 @@ proof -
    and gsCNodes:
     "\<And>a n. (\<exists>cs. kheap s a = Some (CNode n cs) \<and> well_formed_cnode_n n cs) \<longleftrightarrow>
             gsCNodes s' a = Some n"
-   and gsPTs:
-    "\<And>a pt_t. (\<exists>pt. kheap s a = Some (ArchObj (PageTable pt)) \<and> pt_t = pt_type pt) \<longleftrightarrow>
-               gsPTTypes (ksArchState s') a = Some pt_t"
     by (fastforce simp add: ghost_relation_def)+
 
   show "?thesis"
@@ -250,7 +234,7 @@ proof -
       apply simp
      apply (rename_tac arch_kernel_obj)
      apply (case_tac arch_kernel_obj; simp add: image_def)
-      apply (erule allE, drule_tac x=0 in bspec, simp, fastforce)
+      apply (erule_tac x=0 in allE, simp)
      apply (erule_tac x=0 in allE, simp add: not_less)
      apply (rename_tac vmpage_size)
      apply (case_tac vmpage_size; simp add: bit_simps)
@@ -334,7 +318,6 @@ proof -
         apply (rule conjI, clarsimp simp add: word_gt_0)
         apply (erule n_less_2p_pageBitsForSize)
        apply (clarsimp simp: shiftl_t2n mult_ac)
-      (* TCB *)
       apply (erule pspace_dom_relatedE[OF _ pspace_relation])
       apply (case_tac ko, simp_all add: tcb_relation_cut_def other_obj_relation_def)
         apply (clarsimp simp add: cte_relation_def split: if_split_asm)
@@ -357,12 +340,9 @@ proof -
                        split: option.splits)
       using valid_objs[simplified valid_objs_def Ball_def dom_def fun_app_def]
       apply (erule_tac x=y in allE)
-      using arch_state_relation valid_cur_fpu[simplified valid_cur_fpu_def]
-      apply (erule_tac x=y in allE)
       apply (clarsimp simp add: cap_relation_imp_CapabilityMap valid_obj_def
                                 valid_tcb_def ran_tcb_cap_cases valid_cap_def2
-                                arch_tcb_relation_imp_ArchTcbMap arch_state_relation_def
-                                is_tcb_cur_fpu_def obj_at_def)
+                                arch_tcb_relation_imp_ArchTcbMap)
      apply (simp add: absCNode_def cte_map_def)
      apply (erule pspace_dom_relatedE[OF _ pspace_relation])
      apply (case_tac ko, simp_all add: tcb_relation_cut_def other_obj_relation_def
@@ -438,176 +418,86 @@ proof -
     apply (case_tac arch_kernel_object, simp_all add: absHeapArch_def
                                             split: asidpool.splits)
 
-      apply (in_case "KOASIDPool ?pool")
-      apply clarsimp
-      apply (case_tac arch_kernel_obj)
-         apply (simp add: other_aobj_relation_def asid_pool_relation_def
-                          inv_def o_def)
-        apply (clarsimp simp add:  pte_relation_def)
-       apply (clarsimp simp: other_aobj_relation_def split: if_split_asm)
-      apply (simp add: other_aobj_relation_def)
+     apply clarsimp
+     apply (case_tac arch_kernel_obj)
+       apply (simp add: other_aobj_relation_def asid_pool_relation_def
+                        inv_def o_def)
+      apply (clarsimp simp add:  pte_relation_def)
+     apply (clarsimp split: if_split_asm)+
 
-     apply (in_case "KOPTE ?pte")
-     apply (case_tac arch_kernel_obj;
-            simp add: other_obj_relation_def other_aobj_relation_def asid_pool_relation_def inv_def o_def)
+    apply (case_tac arch_kernel_obj)
+      apply (simp add: other_aobj_relation_def asid_pool_relation_def inv_def
+                       o_def)
+    using pspace_aligned[simplified pspace_aligned_def Ball_def dom_def]
+     apply (erule_tac x=y in allE)
+     apply (clarsimp simp add: pte_relation_def absPageTable_def absPageTable0_def
+                               bit_simps)
+     apply (rule conjI)
+      prefer 2
       apply clarsimp
-      apply (rename_tac p pte pt idx)
-      apply (frule pspace_alignedD, rule pspace_aligned)
-      apply (clarsimp simp add: pte_relation_def)
-      apply (prop_tac "pt_at (pt_type pt) p s", simp add: obj_at_def)
+      apply (rule sym)
+      apply (rule pspace_aligned_distinct_None'
+                  [OF pspace_aligned pspace_distinct], (simp add: bit_simps)+)
+      apply (cut_tac x=ya and n="2^12" in
+             ucast_less_shiftl_helper'[where 'a=machine_word_len and a=3,simplified word_bits_conv], simp+)
+      apply (clarsimp simp add: word_gt_0)
+      apply (rename_tac p p' pt pte off)
+      apply (prop_tac "pt_at p s", simp add: obj_at_def)
       apply (drule page_table_at_cross[OF _ pspace_aligned pspace_distinct pspace_relation])
-      apply (clarsimp simp: page_table_at'_def typ_at'_def ko_wp_at'_def)
-      apply (cut_tac a=p and pt_t="pt_type pt" in gsPTs, clarsimp)
-      apply (case_tac "pt_type pt"; clarsimp)
-       apply (in_case "VSRootPT_T")
-       apply (clarsimp simp: absPageTable_def split del: if_split split: option.splits)
-       apply (rule conjI, clarsimp)
-        apply (rule sym)
-        apply (rule pspace_aligned_distinct_None'[OF pspace_aligned pspace_distinct], assumption)
-        apply simp
-        apply (case_tac "idx << pte_bits = 0", simp)
-        apply (clarsimp simp: word_neq_0_conv)
-        apply (rule shiftl_less_t2n)
-         apply (simp add: table_size_def le_mask_iff_lt_2n[THEN iffD1])
-        apply (simp add: table_size_bounded[unfolded word_bits_def, simplified])
-       apply (clarsimp split del: if_split)
-       apply (prop_tac "idx << pte_bits = 0")
-        apply (rename_tac pt_t')
-        apply (cut_tac a="p + (idx << pte_bits)" and pt_t=pt_t' in gsPTs)
-        apply clarsimp
-        apply (rule ccontr)
-        apply (drule_tac y="idx << pte_bits" in pspace_aligned_distinct_None'
-                                                [OF pspace_aligned pspace_distinct])
-         apply (clarsimp simp: word_neq_0_conv table_size_def)
-         apply (rule shiftl_less_t2n, simp)
-          apply (erule order_le_less_trans)
-          apply (simp add: mask_def bit_simps)
-         apply (simp add: bit_simps)
-        apply simp
-       apply (thin_tac "pte_relation' pte pte'" for pte pte')
-       apply (clarsimp simp: pt_bits_def)
-       apply (case_tac pt; clarsimp)
-       apply (rename_tac vs)
-       apply (clarsimp simp: absPageTable0_def)
-       apply (rule conjI, clarsimp)
-        apply (rule ext, rename_tac offs)
-        apply (erule_tac x="ucast offs" in allE, erule impE, rule ucast_leq_mask)
-         apply (simp add: bit_simps)
-        apply (clarsimp dest!: koTypeOf_pte simp: objBits_simps)
-        apply (erule_tac x="ucast offs" in allE)
-        apply clarsimp
-        apply (rename_tac pte y)
-        apply (frule pspace_relation_absD, rule pspace_relation)
-        apply clarsimp
-        apply (drule_tac x="ucast offs" in bspec)
-         apply clarsimp
-         apply (rule ucast_leq_mask)
-         apply (clarsimp simp: bit_simps)
-        apply (clarsimp simp: pte_relation_def ucast_ucast_mask ge_mask_eq vs_index_bits_def)
-        apply (erule pspace_valid_objsE, rule valid_objs)
-        apply (clarsimp simp: valid_obj_def)
-        apply (erule_tac x=offs in allE)
-        apply (clarsimp simp: wellformed_pte_def)
-        apply (case_tac "vs offs"; clarsimp split: if_split_asm)
-         apply (rule set_eqI, simp)
-         apply (rename_tac x, case_tac x; simp)
-        apply (simp add: ucast_ucast_mask ge_mask_eq)
-        apply clarsimp
-        apply (erule_tac x="ucast off" in allE)
-        apply (erule impE)
-         apply (rule ucast_leq_mask)
-         apply (clarsimp simp: bit_simps)
-        apply (clarsimp dest!: koTypeOf_pte simp: objBits_simps)
-        apply (frule pspace_relation_absD, rule pspace_relation)
-        apply clarsimp
-        apply (drule_tac x="ucast off" in bspec)
-         apply clarsimp
-         apply (rule ucast_leq_mask)
-         apply (clarsimp simp: bit_simps)
-        apply (clarsimp simp: pte_relation_def ucast_ucast_mask ge_mask_eq vs_index_bits_def)
-        apply (case_tac "vs off"; simp add: ucast_leq_mask ppn_len_val)
-
-      (* NormalPT_T is an exact duplicate of the VSRootPT_T case, but I don't see any good way
-         to factor out the commonality *)
-      apply (in_case "NormalPT_T")
-      apply (clarsimp simp: absPageTable_def split del: if_split split: option.splits)
-      apply (rule conjI, clarsimp)
-       apply (rule sym)
-       apply (rule pspace_aligned_distinct_None'[OF pspace_aligned pspace_distinct], assumption)
-       apply simp
-       apply (case_tac "idx << pte_bits = 0", simp)
-       apply (clarsimp simp: word_neq_0_conv)
-       apply (rule shiftl_less_t2n)
-        apply (simp add: table_size_def le_mask_iff_lt_2n[THEN iffD1])
-       apply (simp add: table_size_bounded[unfolded word_bits_def, simplified])
-      apply (clarsimp split del: if_split)
-      apply (prop_tac "idx << pte_bits = 0")
-       apply (rename_tac pt_t')
-       apply (cut_tac a="p + (idx << pte_bits)" and pt_t=pt_t' in gsPTs)
-       apply clarsimp
-       apply (rule ccontr)
-       apply (drule_tac y="idx << pte_bits" in pspace_aligned_distinct_None'
-                                               [OF pspace_aligned pspace_distinct])
-        apply (clarsimp simp: word_neq_0_conv table_size_def)
-        apply (rule shiftl_less_t2n, simp)
-         apply (erule order_le_less_trans)
-         apply (simp add: mask_def bit_simps)
-        apply (simp add: bit_simps)
-       apply simp
-      apply (thin_tac "pte_relation' pte pte'" for pte pte')
-      apply (clarsimp simp: pt_bits_def)
-      apply (case_tac pt; clarsimp)
-      apply (rename_tac vs)
-      apply (clarsimp simp: absPageTable0_def)
-      apply (rule conjI, clarsimp)
-       apply (rule ext, rename_tac offs)
-       apply (erule_tac x="ucast offs" in allE, erule impE, rule ucast_leq_mask)
-        apply (simp add: bit_simps)
-       apply (clarsimp dest!: koTypeOf_pte simp: objBits_simps)
-       apply (erule_tac x="ucast offs" in allE)
-       apply clarsimp
-       apply (rename_tac pte y)
-       apply (frule pspace_relation_absD, rule pspace_relation)
-       apply clarsimp
-       apply (drule_tac x="ucast offs" in bspec)
-        apply clarsimp
-        apply (rule ucast_leq_mask)
-        apply (clarsimp simp: bit_simps)
-       apply (clarsimp simp: pte_relation_def ucast_ucast_mask ge_mask_eq vs_index_bits_def)
-       apply (erule pspace_valid_objsE, rule valid_objs)
-       apply (clarsimp simp: valid_obj_def)
-       apply (erule_tac x=offs in allE)
-       apply (clarsimp simp: wellformed_pte_def)
-       apply (case_tac "vs offs"; clarsimp split: if_split_asm)
-        apply (rule set_eqI, simp)
-        apply (rename_tac x, case_tac x; simp)
-       apply (simp add: ucast_ucast_mask ge_mask_eq)
-      apply clarsimp
-      apply (erule_tac x="ucast off" in allE)
-      apply (erule impE)
-       apply (rule ucast_leq_mask)
+      apply (clarsimp simp: page_table_at'_def typ_at'_def ko_wp_at'_def bit_simps)
+      apply (erule_tac x=off in allE)
+      apply (clarsimp dest!: koTypeOf_pte simp: objBits_simps bit_simps)
+      apply (rename_tac pte')
+      apply (erule pspace_dom_relatedE[OF _ pspace_relation])
+      apply (case_tac ko; simp add: tcb_relation_cut_def other_obj_relation_def)
+       apply (clarsimp simp add: cte_relation_def split: if_split_asm)
+      apply (rename_tac ako' y ko P ako)
+      apply (case_tac ako; clarsimp simp: other_aobj_relation_def bit_simps)
+       apply (simp add: pte_relation_def)
+    using pspace_aligned[simplified pspace_aligned_def Ball_def dom_def]
+       apply (erule_tac x=y in allE)
        apply (clarsimp simp: bit_simps)
-      apply (clarsimp dest!: koTypeOf_pte simp: objBits_simps)
-      apply (frule pspace_relation_absD, rule pspace_relation)
-      apply clarsimp
-      apply (drule_tac x="ucast off" in bspec)
+       apply (drule (2) distinct_word_add_inj_ptes[unfolded bit_simps])
        apply clarsimp
-       apply (rule ucast_leq_mask)
-       apply (clarsimp simp: bit_simps)
-      apply (clarsimp simp: pte_relation_def ucast_ucast_mask ge_mask_eq vs_index_bits_def)
-      apply (case_tac "vs off"; simp add: ucast_leq_mask ppn_len_val)
-
-     apply (in_case "DataPage ?p ?sz")
-     apply (clarsimp split: if_splits)
-
-    apply (in_case "KOVCPU ?vcpu")
-    apply clarsimp
-    apply (rename_tac arch_kernel_obj vcpu)
-    apply (case_tac arch_kernel_obj;
-           clarsimp simp: other_obj_relation_def other_aobj_relation_def pte_relation_def split: if_splits)
-    apply (rename_tac vcpu')
-    apply (case_tac vcpu')
-    apply (clarsimp simp: vcpu_relation_def split: vcpu.splits)
+       apply (rename_tac pt)
+       apply (case_tac "pt off"; simp add: ppn_len_def ucast_leq_mask)
+    using pspace_aligned[simplified pspace_aligned_def Ball_def dom_def]
+      apply (erule_tac x=y in allE)
+      apply clarsimp
+      apply (case_tac "n = 0", simp split: if_split_asm)
+      apply (prop_tac "p = y + ((n << pageBits) - (ucast off << pte_bits))")
+       apply (clarsimp simp: field_simps bit_simps)
+      apply simp
+      apply (case_tac "(n << pageBits) - (ucast off << pte_bits) = 0", simp)
+      apply (drule_tac x=y and y="(n << pageBits) - (ucast off << pte_bits)" in
+                       pspace_aligned_distinct_None'[OF pspace_aligned pspace_distinct])
+       prefer 2
+       apply simp
+      apply (clarsimp simp: bit_simps)
+      apply (rule conjI)
+       apply (rule neq_le_trans; clarsimp)
+      apply (erule (1) pte_offset_in_datapage[unfolded bit_simps])
+     apply clarsimp
+     apply (subgoal_tac "ucast ya << 3 = 0")
+      prefer 2
+      apply (rule ccontr)
+      apply (frule_tac x=y in unaligned_helper, assumption)
+       apply (rule ucast_less_shiftl_helper'[where a=3], simp_all)
+     apply (rule ext)
+     apply (frule pspace_relation_absD[OF _ pspace_relation])
+     apply simp
+     apply (erule_tac x=off in allE)+
+     apply (clarsimp simp add: pte_relation_def bit_simps)
+    using valid_objs[simplified valid_objs_def fun_app_def dom_def, simplified]
+     apply (erule_tac x=y in allE)
+     apply (clarsimp simp add: valid_obj_def wellformed_pte_def)
+     apply (erule_tac x=off in allE)
+     apply (case_tac "pt off"; clarsimp simp add: ucast_down_ucast_id is_down split: if_splits)
+      apply (rule set_eqI, clarsimp)
+      apply (case_tac x; simp)
+     apply (rule set_eqI, clarsimp)
+     apply (case_tac x; simp)
+    apply (clarsimp split: if_splits)
     done
 qed
 
